HMAC_isPRF contains propositional def of crypto prperty, plus the proof (complete, apart from non-injectivity of bitsToBytes) proof of injectivity of splitAndPad

sha/HMAC_equivalence.v
@@ -1,6 +1,7 @@
 Require Import Coqlib.
 Require Import Bvector.
 Require Import List.
+Require Import Integers.
 Require Import BinNums.
 (*Require Import Arith.*)
 Require Import common_lemmas.
@@ -24,6 +25,202 @@ Lemma of_length_proof_irrel n a: forall M,
 Proof. intros.
   unfold of_list_length. destruct M. apply Vector.to_list_of_list_opp. 
 Qed.
+
+(***** TODO: move the following lemmas to hmac_purelemmas, or to some Coqlib file*******)
+Lemma app_inv_length1 {A}: forall (l1 m1 l2 m2:list A),
+  l1++l2 = m1++m2 -> length l1 = length m1 -> l1=m1 /\ l2=m2.
+Proof.
+induction l1; simpl; intros.
+{ destruct m1; simpl in *. split; trivial. omega. }
+{ destruct m1; simpl in *. discriminate.
+  inversion H; clear H; subst a0.
+  destruct (IHl1 _ _ _ H3). omega.
+  subst. split; trivial. }
+Qed.
+
+Lemma app_inv_length2 {A}: forall (l1 m1 l2 m2:list A),
+  l1++l2 = m1++m2 -> length l2 = length m2 -> l1=m1 /\ l2=m2.
+Proof.
+induction l1; simpl; intros.
+{ destruct m1; simpl in *. split; trivial.
+  assert (length l2 = length (a :: m1 ++ m2)). rewrite <- H; trivial.
+  rewrite H1 in H0; clear H H1. simpl in H0. rewrite app_length in H0. omega. }
+{ assert (length (a :: l1 ++ l2) = length (m1 ++ m2)). rewrite <- H; trivial.
+  simpl in H1. do 2 rewrite app_length in H1. rewrite H0 in H1.
+  destruct m1; simpl in *. omega.
+  inversion H; clear H. subst a0.
+  destruct (IHl1 _ _ _ H4 H0). subst. split; trivial. }
+Qed.
+
+Lemma cons_inv {A}: forall (a1 a2:A) t1 t2, a1::t1 = a2::t2 -> a1=a2 /\ t1=t2.
+  intros. inversion H; split; trivial. Qed.
+
+Lemma mod_exists a b c: a mod b = c -> b<> 0 -> exists k, k*b+c=a.
+Proof. intros. specialize (Zmod_eq_full a b H0). intros.
+  exists (a/b). rewrite H in H1; clear H H0. subst c. omega. Qed.
+
+Lemma Forall2_map {A B} (f:A -> B): forall l m, 
+      Forall2 (fun x y => y = f x) l m -> map f l = m.
+Proof. intros.
+  induction H; simpl. reflexivity.
+  subst y. f_equal. trivial.
+Qed.
+
+Lemma app_inj1 {A} l2 m2: forall (l1 m1:list A) (H:l1++l2=m1++m2),
+      length l1=length m1 -> l1=m1 /\ l2=m2.
+Proof. induction l1.
+  destruct m1; simpl; intros. split; trivial. discriminate.
+  destruct m1; simpl; intros. discriminate.
+  inversion H; subst. 
+  destruct (IHl1 _ H3). omega.
+  subst. split; trivial.
+Qed.
+
+(********************************************************************************)
+
+Lemma pad_injective_aux (l1 l2: list Z) k 
+     (K : k * Int.modulus + (BlockSize + Zlength l1) * 8 =
+          (BlockSize + Zlength l2) * 8)
+     (N : k <> 0):
+     - (BlockSize + Zlength l2 + 9) mod 64 = - (BlockSize + Zlength l1 + 9) mod 64.
+Proof. repeat rewrite <- Z.add_assoc. unfold BlockSize.
+         repeat rewrite Z.opp_add_distr. 
+         rewrite (Zplus_mod (-(64))).
+         assert (- (64) mod 64 = 0). reflexivity. rewrite H.
+         rewrite (Zplus_mod (-(64))). rewrite H. simpl.
+         repeat rewrite Zmod_mod.
+         rewrite Zplus_mod. rewrite (Zplus_mod (- Zlength l1)). 
+         assert (Z12: - Zlength l2 mod 64 = - Zlength l1 mod 64).
+         { clear H. repeat rewrite Z.mul_add_distr_r in K.
+           assert (k * Int.modulus + Zlength l1 * 8 = Zlength l2 * 8). omega.
+           clear K.
+           assert (KK: k * (Int.modulus/8) + Zlength l1 = Zlength l2).
+              rewrite <- (Zdiv_unique (k * Int.modulus + Zlength l1 * 8) 8 (Zlength l2) 0).
+              2: rewrite Z.add_0_r; trivial. 2: omega.
+              clear H. remember (Zlength l1) as z; clear Heqz. 
+              remember ((Int.modulus / 8)).
+              assert (Int.modulus = z0 * 8). subst. 
+                rewrite <- initialize.max_unsigned_modulus.
+                rewrite client_lemmas.int_max_unsigned_eq. simpl. trivial.
+              rewrite H; clear H Heqz0. rewrite Z.mul_assoc.
+              rewrite (Z_div_plus_full_l (k*z0) 8 (z*8)). 2: omega. 
+              rewrite Z_div_mult_full. trivial. omega.
+           rewrite <- KK; clear H KK.
+           rewrite Z.opp_add_distr.  
+           rewrite Zplus_mod.
+           assert (KM: - (k * (Int.modulus / 8)) mod 64 = 0).
+             apply Zmod_unique with (a:=-k * 8388608). 2: omega. rewrite Zplus_0_r.
+             rewrite <- initialize.max_unsigned_modulus.
+             rewrite client_lemmas.int_max_unsigned_eq. simpl.
+             rewrite Zopp_mult_distr_l, <- Z.mul_assoc. reflexivity.
+           rewrite KM. simpl. apply Z.mod_mod. omega.
+         } 
+         rewrite Z12; trivial.
+Qed. 
+
+Lemma pad_injective_Case5 l1 l2
+  (H0 : (l1 ++ 128 :: nil) ++
+        list_repeat (Z.to_nat (- (BlockSize + Zlength l1 + 9) mod 64)) 0 =
+        (l2 ++ 128 :: nil) ++
+        list_repeat (Z.to_nat (- (BlockSize + Zlength l2 + 9) mod 64)) 0)
+  (H : (BlockSize + Zlength l1) * 8 =
+       ((BlockSize + Zlength l2) * 8) mod Int.modulus)
+  (Nonneg1 : 0 <= (BlockSize + Zlength l1) * 8)
+  (l : (BlockSize + Zlength l1) * 8 < Int.modulus):
+  length l1 = length l2.
+Proof. symmetry in H.
+       destruct (mod_exists _ _ _ H) as [k K].
+       specialize Int.modulus_pos; intros; omega.
+       destruct (zeq k 0). 
+         subst. clear - K. 
+         assert (Zlength l1 = Zlength l2). omega.
+         repeat rewrite Zlength_correct in H.
+         rewrite <- (Nat2Z.id (length l1)).
+         rewrite <- (Nat2Z.id (length l2)).
+         rewrite H. reflexivity.
+       clear H.
+       assert (length ((l1 ++ 128 :: nil) ++
+                list_repeat (Z.to_nat (- (BlockSize + Zlength l1 + 9) mod 64)) 0) 
+             = length ((l2 ++ 128 :: nil) ++
+                list_repeat (Z.to_nat (- (BlockSize + Zlength l2 + 9) mod 64)) 0)).
+       rewrite H0; trivial.
+       clear H0. repeat rewrite app_length in H.
+       repeat rewrite length_list_repeat in H.
+       clear - K n H.
+       rewrite (pad_injective_aux l1 l2 k K n) in H. omega.
+Qed. 
+
+Lemma pad_inc_injective: forall l1 l2, pad_inc l1 = pad_inc l2 -> l1=l2.
+Proof. intros.
+remember (beq_nat (length l1) (length l2)).
+destruct b.
+{ apply beq_nat_eq in Heqb. 
+  unfold pad_inc in H. repeat rewrite Zlength_correct in H.
+  rewrite <- Heqb in H.
+  eapply app_inv_tail. apply H. }
+{ symmetry in Heqb; apply beq_nat_false in Heqb.
+  unfold pad_inc in H.
+  repeat rewrite app_assoc in H.
+  destruct (app_inv_length2 _ _ _ _ H); clear H. reflexivity.
+  apply pure_lemmas.intlist_to_Zlist_inj in H1.
+  apply cons_inv in H1. destruct H1 as [_ Y].
+  apply cons_inv in Y. destruct Y as [Y _].
+  assert (Int.unsigned (Int.repr ((BlockSize + Zlength l1) * 8)) = Int.unsigned (Int.repr ((BlockSize + Zlength l2) * 8))).
+    rewrite Y; trivial.
+  elim Heqb; clear Heqb Y.
+  repeat rewrite Int.unsigned_repr_eq in H.
+  assert (Nonneg1: 0 <= (BlockSize + Zlength l1) * 8).
+    specialize (Zlength_nonneg l1). intros; unfold BlockSize; omega.
+  assert (Nonneg2: 0 <= (BlockSize + Zlength l2) * 8).
+    specialize (Zlength_nonneg l2). intros; unfold BlockSize; omega.
+  remember (zlt ((BlockSize + Zlength l1) * 8) Int.modulus).
+  destruct s; clear Heqs.
+  {  rewrite Zmod_small in H. 2: split; assumption.
+     remember (zlt ((BlockSize + Zlength l2) * 8) Int.modulus).
+     destruct s; clear Heqs.
+     { (*Case 3*)
+       rewrite Zmod_small in H. 2: split; assumption.
+       clear - H. 
+       assert (Zlength l1 = Zlength l2). omega.
+       repeat rewrite Zlength_correct in H0.
+       rewrite <- (Nat2Z.id (length l1)).
+       rewrite <- (Nat2Z.id (length l2)).
+       rewrite H0. reflexivity. }
+     { (*Case 5*) clear g Nonneg2.
+       apply pad_injective_Case5; assumption. } }
+  { clear g Nonneg1.
+    remember (zlt ((BlockSize + Zlength l2) * 8) Int.modulus).
+    destruct s; clear Heqs.
+    { (*Case 5, symmetric version*)
+       rewrite (Zmod_small ((BlockSize + Zlength l2) * 8)) in H. 2: split; assumption.
+       symmetry. symmetry in H. symmetry in H0.
+       apply pad_injective_Case5; assumption. }
+    { clear Nonneg2 g.   
+      remember ((BlockSize + Zlength l1) * 8) as z1. 
+      remember ((BlockSize + Zlength l2) * 8) as z2. 
+  
+      rewrite Zmod_eq in H. 2: apply Int.modulus_pos. remember (z1 / Int.modulus) as k1; clear Heqk1.
+      rewrite Zmod_eq in H. 2: apply Int.modulus_pos. remember (z2 / Int.modulus) as k2; clear Heqk2.
+      destruct (zeq k1 k2).
+      { subst. clear -H.
+        assert (Zlength l1 = Zlength l2). omega.
+        repeat rewrite Zlength_correct in H0.
+        rewrite <- (Nat2Z.id (length l1)).
+        rewrite <- (Nat2Z.id (length l2)).
+        rewrite H0. reflexivity. }
+      { assert (length ((l1 ++ 128 :: nil) ++
+                 list_repeat (Z.to_nat (- (BlockSize + Zlength l1 + 9) mod 64)) 0) 
+              = length ((l2 ++ 128 :: nil) ++
+                 list_repeat (Z.to_nat (- (BlockSize + Zlength l2 + 9) mod 64)) 0)).
+          rewrite H0; trivial.
+        clear H0. repeat rewrite app_length in H1.
+        repeat rewrite length_list_repeat in H1.
+        rewrite (pad_injective_aux l2 l1 (k1-k2)) in H1.
+          omega. 
+          rewrite Z.mul_sub_distr_r; omega.
+          omega. } } } }
+Qed.
+  
 
 Section EQUIV.
 
@@ -52,7 +249,7 @@ Qed.
 
 Lemma opad_length:
   length (bytesToBits (HP.HMAC_SHA256.sixtyfour
-                       (Integers.Byte.unsigned HP.Opad))) = HMAC_spec_abstract.b.
+                       (Integers.Byte.unsigned HP.Opad))) = b.
 Proof. rewrite bytesToBits_len, length_SF. reflexivity. Qed. 
  
 Definition opad_v: Bvector b := of_list_length _ _ _ opad_length.
@@ -101,34 +298,6 @@ Proof. reflexivity. Qed.
 Lemma splitAndPad_aux_nil m M: m=nil -> splitAndPad_aux m M= nil.
 Proof. intros; subst. reflexivity. Qed.
 
-Definition splitAndPad_v (m: Blist): list (Bvector b).
-  apply (splitAndPad_aux (toBlocks (sha_splitandpad_inc m))).
-  apply InBlocks_Forall_512. apply sha_splitandpad_inc_InBlocks.
-Defined.
-
-Lemma splitAndPad_nil: exists pf,
-  splitAndPad_v nil = 
-  cons (of_list_length bool 512 (sha_splitandpad_inc nil) pf) nil. 
-Proof. unfold splitAndPad_v. 
-  remember (InBlocks_Forall_512 (sha_splitandpad_inc_InBlocks nil)). clear Heqf.
-  remember (toBlocks (sha_splitandpad_inc nil)).
-  rewrite toBlocks_equation in Heql.
-  remember (sha_splitandpad_inc nil) as m.
-  destruct m. exfalso. clear Heql f l.
-    unfold sha_splitandpad_inc in Heqm. 
-    assert (@length bool nil = length (bytesToBits (pad_inc (bitsToBytes nil)))).
-      rewrite <- Heqm; trivial.
-    simpl in H; clear Heqm. omega.
-  rewrite leb_correct_conv in Heql.
-    2: rewrite Heqm; simpl; omega.
-  rewrite firstn_same in Heql.
-    2: rewrite Heqm; simpl; omega.
-  rewrite skipn_short in Heql.
-    2: rewrite Heqm; simpl; omega.
-  rewrite toBlocks_equation in Heql. subst l.
-  simpl. eexists. reflexivity.
-Qed.
-
 Lemma length_splitandpad_inner_aux: forall ssm pf,
   Forall2
   (fun (bv : Vector.t bool b) (bl : list bool) => bl = Vector.to_list bv)
@@ -154,13 +323,40 @@ Proof.
       remember (toBlocks (skipn 512 (b :: ssm))) as yy.
       clear - Heql. inversion Heql. trivial. }
 Qed.
-    
+
+Definition splitAndPad_v (m: Blist): list (Bvector b).
+  apply (splitAndPad_aux (sha_splitandpad_blocks m)).
+  apply InBlocks_Forall_512. apply sha_splitandpad_inc_InBlocks.
+Defined.
+
+Lemma splitAndPad_nil: exists pf,
+  splitAndPad_v nil = 
+  cons (of_list_length bool 512 (sha_splitandpad_inc nil) pf) nil. 
+Proof. unfold splitAndPad_v, sha_splitandpad_blocks.
+  remember (InBlocks_Forall_512 (sha_splitandpad_inc_InBlocks nil)). clear Heqf.
+  remember (toBlocks (sha_splitandpad_inc nil)).
+  rewrite toBlocks_equation in Heql.
+  remember (sha_splitandpad_inc nil) as m.
+  destruct m. exfalso. clear Heql f l.
+    unfold sha_splitandpad_inc in Heqm. 
+    assert (@length bool nil = length (bytesToBits (pad_inc (bitsToBytes nil)))).
+      rewrite <- Heqm; trivial.
+    simpl in H; clear Heqm. omega.
+  rewrite leb_correct_conv in Heql.
+    2: rewrite Heqm; simpl; omega.
+  rewrite firstn_same in Heql.
+    2: rewrite Heqm; simpl; omega.
+  rewrite skipn_short in Heql.
+    2: rewrite Heqm; simpl; omega.
+  rewrite toBlocks_equation in Heql. subst l.
+  simpl. eexists. reflexivity.
+Qed.
+
 Lemma length_splitandpad_inner m :
    Forall2
      (fun (bv : Vector.t bool b) (bl : list bool) => bl = Vector.to_list bv)
      (splitAndPad_v m) (sha_splitandpad_blocks m).
 Proof. apply length_splitandpad_inner_aux. Qed.
-
 
 (* Note implicit assumption that the key is of the right length
    is now OK, since we're comapring to HP.HMAC_SHA256.HmacCore, not HMAC. *)
@@ -228,7 +424,6 @@ Proof.
   { apply bytes_bits_comp_ind. 
     apply pure_lemmas.Forall_list_repeat. unfold HP.Ipad. omega.
     apply of_length_proof_irrel. }
+
 Qed.
-
-
 End EQUIV.
