sha/HMAC_isPRF.v
@@ -1,0 +1,270 @@
+Require Import Coqlib.
+Require Import Bvector.
+Require Import List.
+Require Import Integers.
+Require Import BinNums.
+(*Require Import Arith.*)
+Require Import common_lemmas.
+Require Import HMAC_functional_prog.
+Require Import ByteBitRelations.
+Require Import hmac_pure_lemmas.
+Require Import hmac_common_lemmas.
+Require Import HMAC_spec_list.
+Require Import HMAC_spec_abstract.
+Require Import HMAC_common_defs.
+Require Import sha_padding_lemmas.
+Require Import SHA256.
+Require Import pure_lemmas.
+Require Import HMAC_equivalence.
+
+Lemma splitAndPad_v_to_sha_splitandpad_blocks l:
+   map Vector.to_list (splitAndPad_v l) = sha_splitandpad_blocks l.
+Proof. apply Forall2_map. apply length_splitandpad_inner. Qed.
+
+Lemma splitAndPad_v_eq_inverse: forall l m, splitAndPad_v l = splitAndPad_v m ->
+      sha_splitandpad_blocks l = sha_splitandpad_blocks m.
+Proof. intros. do 2 rewrite <- splitAndPad_v_to_sha_splitandpad_blocks.
+  rewrite H. trivial.
+Qed. 
+
+Lemma toBlocks_injective: forall l1 l2 (BLKS: toBlocks l1 = toBlocks l2)
+     (F1: InBlocks 512 l1)
+     (F2: InBlocks 512 l2), l1 = l2.
+Proof.
+ intros l1. 
+  remember (toBlocks l1). generalize dependent l1.
+  induction l. simpl; intros.
+    rewrite toBlocks_equation in *.
+    destruct l1.
+      destruct l2; trivial.
+      destruct (Compare_dec.leb (length (b :: l2)) 511); discriminate.
+    destruct (Compare_dec.leb (length (b :: l1)) 511); discriminate.
+
+  intros.
+    rewrite toBlocks_equation in Heql, BLKS.
+    destruct l1; try discriminate. destruct l2; try discriminate.
+    inversion F1; clear F1. rewrite H0 in Heql.
+    assert (L1: (511 < length (front ++ back))%nat).
+      rewrite app_length, H. omega.
+    rewrite leb_correct_conv in Heql; trivial.
+    rewrite firstn_exact in Heql; trivial.
+    rewrite skipn_exact in Heql; trivial.
+    apply cons_inv in Heql; destruct Heql. subst a l.
+
+    inversion F2; clear F2. rewrite H4 in BLKS. 
+    assert (L2: (511 < length (front0 ++ back0))%nat).
+      rewrite app_length, H3. omega.
+    rewrite leb_correct_conv in BLKS; trivial.
+    rewrite firstn_exact in BLKS; trivial.
+    rewrite skipn_exact in BLKS; trivial.
+    apply cons_inv in BLKS; destruct BLKS. subst front0 full0 full.
+    specialize (IHl _ H8 _ (eq_refl _) H5 H1). subst back0.
+    rewrite <- H4 in H0. assumption.
+Qed.
+ 
+Lemma bytesToBits_nil_inv l: nil = bytesToBits l -> l = nil.
+Proof. destruct l; trivial. simpl; intros. discriminate. Qed.  
+
+Lemma bytesToBits_cons b l:
+      bytesToBits (b::l) = byteToBits b ++ bytesToBits l.
+Proof. reflexivity. Qed.
+
+Lemma byteToBits_injective: forall a b,
+      byteToBits a = byteToBits b ->
+      isbyteZ a -> isbyteZ b -> a = b. 
+Proof. intros. unfold isbyteZ in *. 
+assert (bitsToByte (byteToBits a) = bitsToByte (byteToBits b)).
+  rewrite H; trivial.
+clear H.
+rewrite byte_bit_byte_id in H2; trivial.
+rewrite byte_bit_byte_id in H2; trivial.
+Qed.
+  
+Lemma bytesToBits_injective: forall b1 b2, bytesToBits b1 = bytesToBits b2 -> 
+      Forall isbyteZ b1 -> Forall isbyteZ b2 -> b1=b2.
+Proof. induction b1.
+  intros; destruct b2; trivial. discriminate.
+  destruct b2. discriminate.
+  do 2 rewrite bytesToBits_cons.
+  intros. destruct (app_inj1 _ _ _ _ H). reflexivity.
+  rewrite (IHb1 _ H3).
+  rewrite (byteToBits_injective _ _ H2). trivial.
+    eapply Forall_inv; eassumption.
+    eapply Forall_inv; eassumption.
+    eapply Forall_tl; eassumption. 
+    eapply Forall_tl; eassumption. 
+Qed.
+
+Lemma IntModulus32: Int.modulus = 2^32. reflexivity. Qed.
+
+Lemma Intsize_monotone a b: 0 <= Int.unsigned (Int.repr a) <= Int.unsigned (Int.repr b) -> 
+                          Int.size (Int.repr a) <= Int.size (Int.repr b).
+Proof. apply Int.Zsize_monotone. Qed.
+  
+Lemma isByte_mono: forall x y, 0<=y<=x -> isbyteZ x -> isbyteZ y.
+Proof. intros. destruct H0. split; omega. Qed.
+
+Lemma isbyteZ_pad_inc l (B:Forall isbyteZ l): Forall isbyteZ (pad_inc l).
+Proof. unfold pad_inc.
+  apply Forall_app. split. trivial. 
+  apply Forall_app. split. constructor. split; omega. trivial.
+  apply Forall_app. split. apply Forall_list_repeat. split; omega.
+  apply isbyte_intlist_to_Zlist.
+Qed.
+
+Lemma splitAndPad_1to1 b1 b2: splitAndPad_v b1 = splitAndPad_v b2 -> b1 = b2.
+Proof. intros.
+  apply splitAndPad_v_eq_inverse in H.
+  unfold sha_splitandpad_blocks in H.
+  apply toBlocks_injective in H; try apply sha_splitandpad_inc_InBlocks.
+  unfold sha_splitandpad_inc in H.
+  apply bytesToBits_injective in H. 
+    apply pad_inc_injective in H. admit. (*Hole: injectivity of bitsToBytes!!*)
+  apply isbyteZ_pad_inc. eapply HMAC_spec_pad.HMAC_Pad.bitsToBytes_isbyteZ. reflexivity.
+  apply isbyteZ_pad_inc. eapply HMAC_spec_pad.HMAC_Pad.bitsToBytes_isbyteZ. reflexivity.
+Qed.
+
+Lemma opad_ne_ipad : opad_v <> ipad_v.
+  intros N. 
+  assert (Vector.to_list opad_v = Vector.to_list ipad_v). rewrite N; trivial.
+  unfold opad_v, ipad_v in H. 
+  repeat rewrite of_length_proof_irrel in H.
+  unfold HP.Opad, HP.Ipad in H. simpl in H.
+  discriminate.
+Qed.
+
+(* A definition of a PRF in the form of a predicate. *)
+Set Implicit Arguments.
+
+Require Import FCF.
+(*Require Import HMAC_spec.*)
+Require Import PRF.
+Require Import NMAC_to_HMAC.
+Require Import hF.
+(*Require Import GHMAC_PRF.
+*)
+Require Import HMAC_PRF.
+
+Definition isPRF {D R Key:Set} (RndKey:Comp Key) (RndR: Comp R) (f: Key -> D -> R) 
+                         (ED:EqDec D) (ER:EqDec R) advantage adversary :=
+        PRF_Advantage RndKey RndR f _ _ adversary <= advantage.
+(*Section HMAC_is_PRF.*)
+Variable tau : Rat.
+Variable epsilon : Rat.
+Variable sigma : Rat.
+Variable A : OracleComp Blist (Bvector c) bool. (*I seem to need this variable here, too*)
+(*Hypothesis*)
+Parameter A_wf : well_formed_oc A.
+
+(* Assume h is a tau-PRF against adversary (PRF_h_A h_star_pad A_GHMAC) *)
+(*Hypothesis*)
+Definition h_PRF := isPRF ({ 0 , 1 }^c) ({ 0 , 1 }^c) h_v (Bvector_EqDec (b c p)) (Bvector_EqDec c) tau 
+                         (PRF_h_A (h_star_pad h_v fpad_v) 
+                                  (HMAC_PRF.A_GHMAC p splitAndPad_v A)).
+
+(* We could make similar predicates for the other definitions, or just
+assume the inequalities*)
+(*Hypothesis*)
+Definition h_star_WCR := cAU.Adv_WCR (list_EqDec (Bvector_EqDec (b c p)))
+             (Bvector_EqDec (b c p)) (h_star_pad h_v fpad_v)
+       ({ 0 , 1 }^c) (au_F_A (A_GHMAC p splitAndPad_v A)) <= epsilon.
+
+(*Hypothesis*)
+Definition dual_h_RKA :=
+    RKA_Advantage _ _ _ ({ 0 , 1 }^b c p) ({ 0 , 1 }^c) (dual_f h_v) (BVxor (b c p))
+      (HMAC_RKA_A h_v iv_v fpad_v opad_v ipad_v (A_GHMAC p splitAndPad_v A)) <= sigma.
+
+Theorem HMAC_isPRF (HH1: h_PRF) (HH2: h_star_WCR) (HH3: dual_h_RKA):
+        isPRF (Rnd (b c p)) (Rnd c) 
+              (HMAC h_v iv_v splitAndPad_v
+                              fpad_v opad_v ipad_v)
+              _ _ (tau + epsilon + sigma) A.
+Proof. unfold isPRF.
+  specialize (HMAC_PRF h_v iv_v splitAndPad_v splitAndPad_1to1
+                              fpad_v opad_ne_ipad A_wf).
+  intros.
+  eapply leRat_trans. apply H. clear H. 
+  unfold h_PRF, isPRF in HH1.
+  unfold HMAC_common_defs.b in *. unfold HMAC_spec.b in *. unfold b in *. unfold GHMAC_PRF.b in *. unfold GNMAC_PRF.b in *.  unfold HMAC_spec.b in *.
+  remember (@PRF_Advantage (Bvector (c + p)) (Bvector c) (Bvector c) ({ 0 , 1 }^c)
+        ({ 0 , 1 }^c) h_v (Bvector_EqDec (c + p)) (Bvector_EqDec c)
+        (@PRF_h_A (c + p) c c (@h_star_pad c p h_v fpad_v)
+           (@A_GHMAC c p splitAndPad_v A))). clear Heqr.
+  unfold h_star_WCR in HH2.
+  unfold HMAC_common_defs.b in *. unfold HMAC_spec.b in *. unfold b in *. unfold GHMAC_PRF.b in *. unfold GNMAC_PRF.b in *.  unfold HMAC_spec.b in *.
+  remember (@cAU.Adv_WCR (Bvector c) (list (Bvector (c + p))) (Bvector (c + p))
+        (@list_EqDec (Bvector (c + p)) (Bvector_EqDec (c + p)))
+        (Bvector_EqDec (c + p)) (@h_star_pad c p h_v fpad_v) ({ 0 , 1 }^c)
+        (@au_F_A (c + p) c (@A_GHMAC c p splitAndPad_v A))).
+  clear Heqr0.
+  unfold dual_h_RKA in HH3.
+  unfold HMAC_common_defs.b in *. unfold HMAC_spec.b in *. unfold b in *. unfold GHMAC_PRF.b in *. unfold GNMAC_PRF.b in *.  unfold HMAC_spec.b in *.
+  remember (@RKA_Advantage (Bvector (c + p)) (Bvector c) (Bvector c)
+        (Bvector (c + p)) (Bvector_EqDec (c + p)) (Bvector_EqDec c)
+        (Bvector_EqDec c) ({ 0 , 1 }^c + p) ({ 0 , 1 }^c)
+        (@dual_f (Bvector c) (Bvector (c + p)) (Bvector c) h_v)
+        (BVxor (c + p))
+        (@HMAC_RKA_A c p h_v iv_v fpad_v opad_v ipad_v
+           (@A_GHMAC c p splitAndPad_v A)) ).
+  clear Heqr1.
+  rewrite ratAdd_comm. 
+  apply ratAdd_leRat_compat; trivial. apply ratAdd_leRat_compat; trivial. (*What's the "omega" tactic for Rat?*)
+Qed.
+
+(*Here's the same stuff but enclosed in a section - but uwhen 
+  closing the section, Coq runs out of memory...
+Section HMAC_is_PRF.
+Variable tau : Rat.
+Variable epsilon : Rat.
+Variable sigma : Rat.
+Variable A : OracleComp Blist (Bvector c) bool. (*I seem to need this variable here, too*)
+Hypothesis A_wf : well_formed_oc A.
+
+(* Assume h is a tau-PRF against adversary (PRF_h_A h_star_pad A_GHMAC) *)
+Hypothesis h_PRF : isPRF ({ 0 , 1 }^c) ({ 0 , 1 }^c) h_v (Bvector_EqDec (b c p)) (Bvector_EqDec c) tau 
+                         (PRF_h_A (h_star_pad h_v fpad_v) 
+                                  (HMAC_PRF.A_GHMAC p splitAndPad_v A)).
+
+(* We could make similar predicates for the other definitions, or just
+assume the inequalities*)
+Hypothesis h_star_WCR : cAU.Adv_WCR (list_EqDec (Bvector_EqDec (b c p)))
+             (Bvector_EqDec (b c p)) (h_star_pad h_v fpad_v)
+       ({ 0 , 1 }^c) (au_F_A (A_GHMAC p splitAndPad_v A)) <= epsilon.
+
+Hypothesis dual_h_RKA :
+    RKA_Advantage _ _ _ ({ 0 , 1 }^b c p) ({ 0 , 1 }^c) (dual_f h_v) (BVxor (b c p))
+      (HMAC_RKA_A h_v iv_v fpad_v opad_v ipad_v (A_GHMAC p splitAndPad_v A)) <= sigma.
+
+Theorem HMAC_isPRF:
+        isPRF (Rnd (b c p)) (Rnd c) 
+              (HMAC h_v iv_v splitAndPad_v
+                              fpad_v opad_v ipad_v)
+              _ _ (tau + epsilon + sigma) A.
+Proof. unfold isPRF.
+  specialize (HMAC_PRF h_v iv_v splitAndPad_v splitAndPad_1to1
+                              fpad_v opad_ne_ipad A_wf).
+  intros.
+  eapply leRat_trans. apply H. clear H. 
+  unfold isPRF in h_PRF.
+  unfold HMAC_common_defs.b in *. unfold HMAC_spec.b in *. unfold b in *. unfold GHMAC_PRF.b in *. unfold GNMAC_PRF.b in *.  unfold HMAC_spec.b in *.
+  remember (@PRF_Advantage (Bvector (c + p)) (Bvector c) (Bvector c) ({ 0 , 1 }^c)
+        ({ 0 , 1 }^c) h_v (Bvector_EqDec (c + p)) (Bvector_EqDec c)
+        (@PRF_h_A (c + p) c c (@h_star_pad c p h_v fpad_v)
+           (@A_GHMAC c p splitAndPad_v A))). clear Heqr.
+  remember (@cAU.Adv_WCR (Bvector c) (list (Bvector (c + p))) (Bvector (c + p))
+        (@list_EqDec (Bvector (c + p)) (Bvector_EqDec (c + p)))
+        (Bvector_EqDec (c + p)) (@h_star_pad c p h_v fpad_v) ({ 0 , 1 }^c)
+        (@au_F_A (c + p) c (@A_GHMAC c p splitAndPad_v A))).
+  clear Heqr0.
+  remember (@RKA_Advantage (Bvector (c + p)) (Bvector c) (Bvector c)
+        (Bvector (c + p)) (Bvector_EqDec (c + p)) (Bvector_EqDec c)
+        (Bvector_EqDec c) ({ 0 , 1 }^c + p) ({ 0 , 1 }^c)
+        (@dual_f (Bvector c) (Bvector (c + p)) (Bvector c) h_v)
+        (BVxor (c + p))
+        (@HMAC_RKA_A c p h_v iv_v fpad_v opad_v ipad_v
+           (@A_GHMAC c p splitAndPad_v A)) ).
+  clear Heqr1.
+  rewrite ratAdd_comm. 
+  apply ratAdd_leRat_compat; trivial. apply ratAdd_leRat_compat; trivial. (*What's the "omega" tactic for Rat?*)
+Qed.
+End HMAC_is_PRF. Runs out of memory*) 
